Examples/tmr/tmr_ft_proof.v
@@ -11,67 +11,63 @@ Open Scope N_scope.
 
 Section Invariants.
     Variable mem : memory.
+    Variable raddr : addr.
     Variable in_a in_b : addr.
     Variable len : N.
+    Variable s0 s1 s2 s3 s4 : N.
 
     Definition k_equal (p1 p2 : addr) (k : N) : Prop :=
         forall (i : N),
             i < k ->
             mem Ⓑ[p1 + i] = mem Ⓑ[p2 + i].
 
-    (* The output of tmr is zero if and only if the two
+    (* The output of CRYPTO_memcmp is zero if and only if the two
        memory regions match up to `len` bytes *)
     Definition postcondition (s : store) : Prop :=
         s R_A0 = 0 <-> k_equal in_a in_b len.
 
     Definition invs T (Inv Post: inv_type T) (NoInv:T) (s:store) (a:addr) : T :=
         match a with
-        | 0x0 => Inv 0
+        (* CRYPTO_memcmp *)
+        | 0x10170 => Inv 0
             (s R_A0 = in_a /\ s R_A1 = in_b /\ s R_A2 = len /\
-              s V_MEM32 = mem)
-        | 0x40 => Inv 0
-            (* Either the invariant is satisfied or we skipped something
-               and all bets are off *)
-            (exists k,
               s V_MEM32 = mem /\
-              s R_A4 = in_a ⊕ k /\
-              s R_A7 = in_b ⊕ k /\
-              s R_A2 = in_a ⊕ len /\
-              s R_A0 = in_a /\ s R_A1 = in_b /\
-              s R_A5 = in_a /\ s R_A6 = in_b /\
-              k < len < 2^32 /\
-              ((s R_T1 = 0) <-> k_equal in_a in_b k)
-            )
-        | 0x60 => Inv 0
-            (exists k,
-              s V_MEM32 = mem /\
-              s R_A0 = in_a ⊕ k /\
-              s R_A1 = in_b ⊕ k /\
-              s R_A2 = in_a ⊕ len /\
-              s R_A5 = in_a /\ s R_A6 = in_b /\
-              k < len < 2^32 /\
-              ((s R_A3 = 0) <-> k_equal in_a in_b k) /\
-              ((s R_T1 = 0) <-> k_equal in_a in_b len)
-            )
-        | 0x80 => Inv 0
+              s R_RA = raddr /\
+              s R_S0 = s0 /\ s R_S1 = s1 /\ s R_S2 = s2 /\
+                s R_S3 = s3 /\ s R_S4 = s4)
+        | 0x10180 => Inv 0
             (exists k,
               s V_MEM32 = mem /\
               s R_A5 = in_a ⊕ k /\
-              s R_A6 = in_b ⊕ k /\
+              s R_A1 = in_b ⊕ k /\
               s R_A2 = in_a ⊕ len /\
               k < len < 2^32 /\
-              ((s R_A1 = 0) <-> k_equal in_a in_b k) /\
-              ((s R_A3 = 0) <-> k_equal in_a in_b len) /\
-              ((s R_T1 = 0) <-> k_equal in_a in_b len)
+              ((s R_A0 = 0) <-> k_equal in_a in_b k) /\
+              s R_RA = raddr /\
+              s R_S0 = s0 /\ s R_S1 = s1 /\ s R_S2 = s2 /\
+                s R_S3 = s3 /\ s R_S4 = s4
             )
-        | 0xdc | 0xe0 => Post 0 (postcondition s)
+        | 0x1019c | 0x101a4 => Post 0 
+            (postcondition s /\ 
+             s R_RA = raddr /\
+             s R_S0 = s0 /\ s R_S1 = s1 /\ s R_S2 = s2 /\
+                s R_S3 = s3 /\ s R_S4 = s4)
+
+        (* passwords_match_tmr *)
+        | 0x101a8 => Inv 1
+            (s R_A0 = in_a /\ s R_A1 = in_b /\ s R_A2 = len /\
+              s V_MEM32 = mem)
+        | 0x102b0 | 0x102b4 => Post 1 (postcondition s)
         | _ => NoInv
         end.
 
-    Definition tmr : program := lift_riscv tmr_ft.
+    Definition tmr_ft : program := lift_riscv tmr_ft.
 
-    Definition exits0 := make_exits 0 tmr invs.
-    Definition invs0 := make_invs 0 tmr invs.
+    Definition exits0 := make_exits 0 tmr_ft invs.
+    Definition invs0 := make_invs 0 tmr_ft invs.
+
+    Definition exits1 := make_exits 1 tmr_ft invs.
+    Definition invs1 := make_invs 1 tmr_ft invs.
 End Invariants.
 
 Lemma k_equal_inv : forall mem a b k,
@@ -104,26 +100,98 @@ Proof.
     now apply N.lxor_eq.
 Qed.
 
-Lemma neq_lxor : forall a b,
-    a <> b -> a .^ b <> 0.
-Proof.
-    intros a b H Contra.
-    apply N.lxor_eq in Contra. contradiction.
-Qed.    
-
 (* Proof in fault-free context *)
-Theorem tmr_correctness:
-  forall s mem t xs' in_a in_b len
-         (ENTRY: startof t xs' = (Addr 0, s))
+Theorem crypto_memcmp_correctness:
+  forall s mem t xs' in_a in_b len raddr s0 s1 s2 s3 s4
+         (ENTRY: startof t xs' = (Addr 0x10170, s))
          (MDL: models rvtypctx s)
          (MEM: s V_MEM32 = mem)
          (A0: s R_A0 = in_a)
          (A1: s R_A1 = in_b)
-         (LEN: s R_A2 = len),
-  satisfies_all tmr (invs0 mem in_a in_b len)
-                    (exits0 mem in_a in_b len) (xs'::t).
+         (LEN: s R_A2 = len)
+         (RA: s R_RA = raddr)
+         (S0: s R_S0 = s0)
+         (S1: s R_S1 = s1)
+         (S2: s R_S2 = s2)
+         (S3: s R_S3 = s3)
+         (S4: s R_S4 = s4),
+  satisfies_all tmr_ft (invs0 mem raddr in_a in_b len s0 s1 s2 s3 s4)
+                       (exits0 mem raddr in_a in_b len s0 s1 s2 s3 s4) (xs'::t).
 Proof using.
     Local Ltac step := time r5_step.
+    intros. apply prove_invs.
+
+    simpl. rewrite ENTRY. step. repeat split; assumption.
+
+    intros.
+    eapply startof_prefix in ENTRY; try eassumption.
+    eapply preservation_exec_prog in MDL; try (eassumption || apply lift_riscv_welltyped).
+    clear - PRE MDL. rename t1 into t. rename s5 into s. rename a1 into a.
+
+    destruct_inv 32 PRE.
+
+    (* Intro *)
+    destruct PRE as (A0 & A1 & A2 & Mem & Saved). {
+    step.
+    - (* len = 0 *)
+        (* apply N.eqb_eq in BC. *)
+        repeat step. repeat split; auto; intuition.
+            unfold k_equal. lia.
+    - (* len <> 0 *)
+        repeat step.
+        exists 0. psimpl; repeat split; auto; intuition.
+        lia. apply (models_var R_A2) in MDL. rewrite <- A2. apply MDL.
+        unfold k_equal. lia.
+    }
+
+    (* Loop *)
+    destruct PRE as (k & Mem & A5 & A1 & A2 & Bound & Eq & Saved). {
+    repeat step.
+    - (* in_a + k + 1 <> in_a + len, loop *)
+        exists (k ⊕ 1). psimpl. repeat split; auto;
+            try solve [intuition]. lia.
+        -- unfold k_equal. intros.
+           apply or_xor_zero in H. destruct H.
+           assert (i < k \/ i = k) by lia. destruct H2.
+               now apply Eq.
+           now subst.
+        -- intros. rewrite N.mod_small in H by lia.
+           pose proof (k_equal_inv _ _ _ _ H). apply Eq in H0.
+           specialize (H k ltac:(lia)).
+           now rewrite H, N.lxor_nilpotent, H0.
+    - (* in_a + k + 1 = in_a + len, break *)
+        assert (1 + k = len) by lia. subst len.
+        repeat split; auto; try solve [intuition]; intro.
+        -- apply or_xor_zero in H. destruct H. rewrite H in *.
+           apply k_equal_step.
+              now apply Eq.
+              now rewrite H0.
+        -- replace (s R_A0) with 0. psimpl.
+           apply N.lxor_eq_0_iff.
+           symmetry. apply H. lia.
+           apply k_equal_inv in H. apply Eq in H.
+           now rewrite H.
+    }
+Qed.
+
+(* Proof in fault-free environment *)
+Theorem tmr_ft_correctness:
+  forall s mem t xs' in_a in_b len raddr s0 s1 s2 s3 s4
+         (ENTRY: startof t xs' = (Addr 0x101a8, s))
+         (MDL: models rvtypctx s)
+         (MEM: s V_MEM32 = mem)
+         (A0: s R_A0 = in_a)
+         (A1: s R_A1 = in_b)
+         (LEN: s R_A2 = len)
+         (RA: s R_RA = raddr)
+         (S0: s R_S0 = s0)
+         (S1: s R_S1 = s1)
+         (S2: s R_S2 = s2)
+         (S3: s R_S3 = s3)
+         (S4: s R_S4 = s4),
+  satisfies_all tmr_ft (invs1 mem raddr in_a in_b len s0 s1 s2 s3 s4)
+                       (exits1 mem raddr in_a in_b len s0 s1 s2 s3 s4) (xs'::t).
+Proof.
     intros. apply prove_invs.
 
     simpl. rewrite ENTRY. step. repeat split; assumption.
@@ -135,120 +203,184 @@ Proof using.
 
     destruct_inv 32 PRE.
 
-    (* Intro 1 *)
-    destruct PRE as (A0 & A1 & A2 & Mem). {
+    (* Intro *)
+    destruct PRE as (A0 & A1 & A2 & Mem).
+    do 20 step.
+    Ltac riscv_call thm :=
+        let MDL1 := fresh "MDL1" in
+        let s1 := fresh "s1" in
+        set (s1 := update _ _ _);
+        eapply models_after_steps;
+        [assumption|apply lift_riscv_welltyped|];
+        intro MDL1; eapply (perform_call 0);
+        [reflexivity|eauto using thm|reflexivity|];
+        let a := fresh "a" in
+        let s' := fresh "s'" in
+        let t2 := fresh "t2" in
+        intros
+            a' s' t2 ENTRY XP UT PRE
+        ; unfold s1 in PRE; psimpl in PRE;
+        let MDL' := fresh "MDL'" in
+        assert (models rvtypctx s') as MDL' by
+            (eapply preservation_exec_prog;
+             eauto using lift_riscv_welltyped);
+        match goal with
+        | [|- context[?t2 ++ ?t0 ++ (Addr ?x, ?s) :: ?t]] =>
+            let t' := fresh "t'" in
+            set (t' := t2++t0++(Addr x, s)::t) in *; clearbody s1;
+            (* repeat match goal with
+            | [PRE: true_inv _ |- _] =>
+                let x := fresh "x" in
+                set (x := s _) in PRE; clearbody x
+            end *)
+            clear - PRE MDL';
+            let MDL := fresh "MDL" in
+            rename MDL' into MDL;
+            destruct_inv 32 PRE
+        end.
+    (* Call CRYPTO_memcmp *)
+    riscv_call crypto_memcmp_correctness.
+
+    - destruct PRE as (Answer1 & RA & S0 & S1 & S2 & S3 & S4).
+      unfold postcondition in Answer1.
+      destruct (N.eq_dec (s' R_A0) 0).
+      -- (* A0 = 0 *)
+        apply Answer1 in e.
+        do 6 step. riscv_call crypto_memcmp_correctness.
+        destruct PRE as (Answer2 & RA & S0 & S1 & S2 & S3 & S4).
+      -- (* A0 <> 0 *)
+        
+         do 6 step;
+         riscv_call crypto_memcmp_correctness.
+
+Section FaultTolerantInvariants.
+    Variable mem : memory.
+    Variable in_a in_b : addr.
+    Variable len : N.
+
+    Definition ft_invs T (Inv Post: inv_type T) (NoInv:T) (s:store) (a:addr) : T :=
+        match a with
+        | 0x0 => Inv 0
+            (s R_A0 = in_a /\ s R_A1 = in_b /\ s R_A2 = len /\
+              s V_MEM32 = mem /\ s V_FC = 1)
+        | 0x28 => Inv 0
+            (exists k,
+              s V_MEM32 = mem /\
+              s R_A5 = in_a ⊕ k /\
+              s R_A1 = in_b ⊕ k /\
+              s R_A2 = in_a ⊕ len /\
+              k < len < 2^32 /\
+              s V_FC <= 1 /\
+              ((s R_A0 = 0) <-> k_equal mem in_a in_b k)
+            )
+        | 0x80 | 0x84 | 0x90 | 0x94 => Post 0 (postcondition mem in_a in_b len s)
+        | _ => NoInv
+        end.
+
+    Definition fault_memcmp := inject_fault memcmp.
+
+    Definition ft_exits0 := make_exits 0 fault_memcmp ft_invs.
+    Definition ft_invs0 := make_invs 0 fault_memcmp ft_invs.
+End FaultTolerantInvariants.
+    
+(* Proof in fault-free context *)
+Theorem crypto_memcmp_ft_correctness:
+  forall s mem t xs' in_a in_b len
+         (ENTRY: startof t xs' = (Addr 0, s))
+         (MDL: models rvtypctx s)
+         (MEM: s V_MEM32 = mem)
+         (A0: s R_A0 = in_a)
+         (A1: s R_A1 = in_b)
+         (LEN: s R_A2 = len)
+         (FC: s V_FC = 1),
+  satisfies_all fault_memcmp
+                       (ft_invs0 mem in_a in_b len)
+                       (ft_exits0 mem in_a in_b len) (xs'::t).
+Proof using.
+    Local Ltac step ::= 
+        match goal with
+        | [s' : store, FC : ?s' V_FC <= 1 |- _] =>
+            let H := fresh "H" in
+            assert (s' V_FC = 0 \/ s' V_FC = 1) as H by lia;
+            clear FC; destruct H
+        | _ => idtac
+        end;
+        time r5_step;
+        repeat match goal with
+        | [n : N, BC : ?n mod 2 = _ |- _] => clear BC n
+        | [s' : store, n : N, 
+            BC : (if 0 <? ?s' V_FC then ?n mod 2 else 0) = _ |- _] => clear BC n
+        | [H: ?x = ?x |- _] => clear H
+        end;
+        try discriminate.
+    intros. apply prove_invs.
+
+    simpl. rewrite ENTRY. step. repeat split; assumption.
+
+    intros.
+    eapply startof_prefix in ENTRY; try eassumption.
+    eapply preservation_exec_prog in MDL; try (eassumption || apply inject_fault_lift_riscv_welltyped).
+    clear - PRE MDL. rename t1 into t. rename s1 into s. rename a1 into a.
+
+    destruct_inv 32 PRE.
+
+    (* Intro *)
+    destruct PRE as (A0 & A1 & A2 & Mem & FC). {
+    Local Ltac solve_inv MDL A2 :=
+        exists 0; psimpl; repeat split; auto;
+            [lia|
+            apply (models_var R_A2) in MDL; rewrite <- A2; apply MDL
+            |lia|unfold k_equal; lia].
     step.
-    - (* len = 0 *)
-        (* apply N.eqb_eq in BC. *)
-        repeat step. split; intro.
-            unfold k_equal. lia.
-            reflexivity.
-    - (* len <> 0 *)
+    - (* len = 0, no fault *)
+        repeat step; split; intro;
+            unfold k_equal; lia.
+    - (* len <> 0, no fault *)
+        repeat (step; [| repeat step; solve_inv MDL A2]); solve_inv MDL A2.
+    - (* fault *) 
         repeat step.
-            discriminate.
-        exists 0. psimpl; repeat split; auto.
-        lia. apply (models_var R_A2) in MDL. rewrite <- A2. apply MDL.
-        unfold k_equal. lia.
+            split; intro; unfold k_equal; lia.
+        solve_inv MDL A2.
     }
 
-    (* Loop 1 *)
-    destruct PRE as (k & Mem & A4 & A7 & A2 & A0 & A1 & A5 & A6 & Bound & Eq). {
+    (* Loop *)
+    destruct PRE as (k & Mem & A5 & A1 & A2 & Bound & FC & Eq). {
+    Local Ltac solve_inv' k Eq :=
+        let X := fresh "X" in
+        let Y := fresh "Y" in
+        let Z := fresh "Z" in
+        let W := fresh "W" in
+        let Inv := fresh "Inv" in
+        let i := fresh "i" in
+        exists (k ⊕ 1); psimpl; repeat split;
+        [lia|lia|lia
+        | unfold k_equal; intros X i Z; apply or_xor_zero in X; destruct X;
+            assert (i < k \/ i = k) as Y by lia; destruct Y;
+            [now apply Eq|now subst]
+        | repeat split; intros W; rewrite N.mod_small in W by lia;
+            pose proof (k_equal_inv _ _ _ _ W) as Inv; apply Eq in Inv;
+            specialize (W k ltac:(lia));
+            now rewrite W, N.lxor_nilpotent, Inv].
+    Local Ltac solve_post k len s Eq :=
+        let X := fresh "H" in
+        let i := fresh "i" in
+        let ILen := fresh "ilen" in
+        let KLen := fresh "klen" in
+        assert (1 + k = len) as KLen by lia;
+        subst len;
+        split; intro X;
+            [apply k_equal_step;
+              apply or_xor_zero in X; destruct X;
+              [apply Eq; assumption|now symmetry]
+            |replace (s R_A0) with 0; psimpl;
+              [apply N.lxor_eq_0_iff; symmetry; apply X; lia
+              |apply k_equal_inv in X; symmetry; apply Eq, X]
+            ].
     repeat step.
-    - (* loop *)
-        exists (k ⊕ 1). psimpl. repeat split; auto. lia. lia.
-        -- unfold k_equal. intros.
-           apply or_xor_zero in H. destruct H.
-           assert (i < k \/ i = k) by lia. destruct H2.
-               now apply Eq.
-           now subst.
-        -- intros. rewrite N.mod_small in H by lia.
-           pose proof (k_equal_inv _ _ _ _ H). apply Eq in H0.
-           specialize (H k ltac:(lia)).
-           now rewrite H, N.lxor_nilpotent, H0.
-    - (* break and go to next one *)
-        exists 0. psimpl. repeat split; auto; intros.
-        lia. lia. unfold k_equal; lia.
-        all: replace len with (1 + k) in * by lia.
-        -- apply or_xor_zero in H. destruct H. rewrite H in *.
-           apply k_equal_step.
-              now apply Eq.
-              now rewrite H0.
-        -- replace (s R_T1) with 0. psimpl.
-           apply N.lxor_eq_0_iff.
-           symmetry. apply H. lia.
-           apply k_equal_inv in H. apply Eq in H.
-           now rewrite H.
+    par: match goal with
+        | [ |- context[exists _, _] ] => solve_inv' k Eq
+        | [ |- context[_ /\ _]] => solve_post k len s Eq
+        | _ => idtac
+        end.
     }
-
-    (* Loop 2 *)
-    destruct PRE as (k & Mem & A0 & A1 & A2 & A5 & A6 & Bound & Eq & Last). {
-    repeat step.
-    - exists (k ⊕ 1). psimpl. repeat (split; auto); try lia.
-        -- unfold k_equal. intros.
-           apply or_xor_zero in H. destruct H.
-           assert (i < k \/ i = k) by lia. destruct H2.
-               now apply Eq.
-           now subst.
-        -- intros. rewrite N.mod_small in H by lia.
-           pose proof (k_equal_inv _ _ _ _ H). apply Eq in H0.
-           specialize (H k ltac:(lia)).
-           now rewrite H, N.lxor_nilpotent, H0.
-    - (* break and go to next one *)
-        exists 0. psimpl. repeat (split; auto); intros.
-        lia. lia. unfold k_equal; lia.
-        all: replace len with (1 + k) in * by lia.
-        -- apply or_xor_zero in H. destruct H. rewrite H in *.
-           apply k_equal_step.
-              now apply Eq.
-              now rewrite H0.
-        -- replace (s R_A3) with 0. psimpl.
-           apply N.lxor_eq_0_iff.
-           symmetry. apply H. lia.
-           apply k_equal_inv in H. apply Eq in H.
-           now rewrite H.
-    }
-
-    (* Loop 3 *)
-    destruct PRE as (k & Mem & A5 & A6 & A2 & Bound & Eq & Last1 & Last2). {
-    repeat step.
-    - exists (k ⊕ 1). psimpl. repeat (split; auto); try lia.
-        -- unfold k_equal. intros.
-           apply or_xor_zero in H. destruct H.
-           assert (i < k \/ i = k) by lia. destruct H2.
-               now apply Eq.
-           now subst.
-        -- intros. rewrite N.mod_small in H by lia.
-           pose proof (k_equal_inv _ _ _ _ H). apply Eq in H0.
-           specialize (H k ltac:(lia)).
-           now rewrite H, N.lxor_nilpotent, H0.
-    - (* exit *)
-        replace len with (1 + k) in * by lia.
-        split; intro.
-        -- destruct N.ltb eqn:E in H. discriminate. clear H.
-            apply N.ltb_ge, N.le_0_r, N.lor_eq_0_iff in E.
-            destruct E.
-            rewrite N.land_lor_distr_r in H, H0.
-            apply N.lor_eq_0_iff in H, H0. destruct H, H0.
-            rewrite N.land_lor_distr_r in H1.
-            apply N.lor_eq_0_iff in H1. destruct H1.
-            destruct (N.eq_dec (s R_T1) 0).
-                rewrite e in *. now apply Last2.
-            destruct (N.eq_dec (s R_A3) 0).
-                rewrite e in *. now apply Last1.
-            destruct (N.eq_dec (s R_A1) 0).
-                rewrite e in *; clear e H1 H0 Last1 Last2.
-                apply k_equal_step. now apply Eq.
-            destruct (N.eq_dec (s R_T1) (s R_A3)).
-                rewrite e in *; clear e.
-                rewrite N.land_diag in H. contradiction.
-            destruct (N.eq_dec (s R_T1) (mem Ⓑ[ in_b + k ] .^ mem Ⓑ[ in_a + k ])).
-                rewrite e in *; clear e.
-                rewrite N.land_diag in H3. contradiction.
-            destruct (N.eq_dec (s R_A3) (mem Ⓑ[ in_b + k ] .^ mem Ⓑ[ in_a + k ])).
-                rewrite e in *; clear e.
-                rewrite N.land_diag in H2. contradiction.
-            (* How the heck do I show that this is a contradiction? *)
-            admit.
-            admit.
-    }
-Admitted.
+Qed.
